* Update on LTS definition

src/formalisms/lts.v
@@ -1,51 +1,105 @@
 (** %\chapter{Labelled Transitionsition System (LTS)}\label{chap::lts}%
 
-  This definition follows the canonical definition of a LTS, see %\cite{gorrieriLabeledTransitionSystems2017a}%
+In this chapter, we define Labelled Transition Systems (or LTS). This definition follows the canonical definition of a _deterministic_ LTS, see %\cite00{gorrieriLabeledTransitionSystems2017a}%. *)
+
+(* begin hide *)
+Require Import Coq.Lists.List.
+Import ListNotations. (* from List *)
+
+Section LTS_Definition.
+(* end hide *)
+
+(** * Definition of LTS
+
+_Notes_:
+- we opted for [bool] rather than [Prop] to allow for on-the-fly evaluation of the LTS.
+- we define both a [LTS_Transition] predicate and a [LTS_Step] function. The step function allows building a simulator, whereas the transition function allows performing proof. We keep the definition of [LTS_Transition] but are likely to remove it ultimately.
 
 *)
 
+  Definition LTS_Transitions (S : Type) (A : Type) := S -> A -> S -> bool.
+
+  Definition LTS_Step (S : Type) (A : Type) := S -> A -> S.
+
+  Record LTS_struct : Type := mkLTS_struct  {
+    States : Type;
+    Init : States;
+    Actions : Type;
+    Steps : LTS_Step States Actions;
+  }.
+
+(** [step_lts] performs one step of the LTS. *)
+
+  Definition step_lts
+    (A_LTS : LTS_struct) (state: States A_LTS) (action : Actions A_LTS) :=
+      (Steps A_LTS) state action.
+
+(** See implementation in [lts.v] for example of use. *)
+
 (* begin hide *)
-Set Asymmetric Patterns.
-Set Implicit Arguments.
-Unset Strict Implicit.
-(* end hide *)
+End LTS_Definition.
 
-(** * Definition of LTS *)
+(* The following could be added to the definition of a LTS *)
+ (* Transitions : LTS_Transitions States Actions;
 
-Definition LTS_Transitions (S : Type) (A : Set) := S -> A -> S -> Prop.
+ XXX But this seems like an unnecessary definition
+ *)
 
-(** We use Coq module to increase the modularity of this formalization.
-  Ultimately, a LTS will be parameterized by States and Actions.
+(*
+Definition Transitions_Steps_Equivalent (A_LTS : LTS_struct) :=
+  forall (state: States A_LTS) (action: Actions A_LTS),
+  exists x: (States A_LTS), In x ((Steps A_LTS) state action) ->
+    (Transitions A_LTS state action x) = true.
 
-  Probably use a record instead XXXX
+Definition step_lts_predicate
+  (A_LTS : LTS_struct) (current_state : States A_LTS)
+  (action : Actions A_LTS) (destination : States A_LTS) :=
+    (Transitions A_LTS) current_state action destination.
+*)
 
-  *)
+(** Example *)
 
-Module Type LTS_struct.
-  Parameter State : Type.
-  Parameter Init : State.
-  Parameter Action : Set.
-  Parameter Transitions : LTS_Transitions State Action.
-End LTS_struct.
+Section Example.
 
-(** * Example *)
+Inductive ab : Set := A | B.
+Inductive ab_actions : Set := ReadA | ReadB | Fail.
 
-Inductive ab := A | B.
+Definition AB_Transitions (s1 : ab) (a: ab_actions) (s2 : ab) : bool :=
+    match s1, a, s2 with
+    | A, _, B => true
+    | B, _, A => true
+    | _, _, _ => false
+    end.
 
-Inductive ab_state : Set := ReadA | ReadB | Fail.
-
-Definition Some_Transitions
-  (s1 : ab) (a: ab_state) (s2 : ab) : Prop
-  :=
-  match s1, a, s2 with
-  | _, _, _ => True
+Definition AB_Steps (s1 : ab) (a: ab_actions) :=
+  match s1, a  with
+  | A, _ => B
+  | B, _ => A
   end.
 
-Module LTS_Test <: LTS_struct.
-  Definition State := ab.
-  Definition Init := A.
-  Definition Action := ab_state.
-  Definition Transitions := Some_Transitions.
-End LTS_Test.
+Definition LTS_Test : LTS_struct := {|
+  States := ab;
+  Init := A;
+  Actions := ab_actions;
+  (*Transitions := AB_Transitions; *)
+  Steps := AB_Steps;
+|}.
 
-Compute LTS_Test.Transitions A ReadA B.
+(*
+Lemma e: Transitions_Steps_Equivalent LTS_Test.
+Proof.
+    unfold Transitions_Steps_Equivalent.
+    intros.
+    induction state.
+    - now exists B.
+    - now exists A.
+Qed.
+*)
+Example f' := step_lts LTS_Test (Init LTS_Test) ReadA.
+Lemma test : f' = B.
+Proof.
+  auto.
+Qed.
+
+End Example.
+(* end hide *)
